Cslib/Computability/LambdaCalculus/WellScoped/FSub/RetypeTheory/TypeSystem.lean
@@ -1,22 +1,19 @@
 import Cslib.Computability.LambdaCalculus.WellScoped.FSub.RetypeTheory.Core
 
+/-- Context retyping preserves subtyping judgments. -/
 def Subtyp.retype {σ : Subst s1 s2}
   (hsub : Subtyp Γ T1 T2)
   (ρ : Retype Γ σ Δ) :
   Subtyp Δ (T1.subst σ) (T2.subst σ) := by
-  induction hsub generalizing s2
-  case top => constructor
-  case refl => constructor
-  case trans ih1 ih2 =>
-    apply Subtyp.trans <;> aesop
-  case tvar hb =>
-    apply ρ.tvar _ _ hb
+  induction hsub generalizing s2 <;> try (solve | constructor)
+  case trans ih1 ih2 => apply Subtyp.trans <;> aesop
+  case tvar hb => apply ρ.tvar _ _ hb
   case arrow => apply arrow <;> aesop
   case poly ih1 ih2 =>
-    apply poly
-    { apply ih1 ρ }
+    apply poly <;> try grind
     { apply ih2 ρ.liftTVar }
 
+/-- Context retyping preserves typing judgments. -/
 theorem HasType.retype {σ : Subst s1 s2}
   (ht : HasType Γ t T)
   (ρ : Retype Γ σ Δ) :
@@ -24,21 +21,9 @@ theorem HasType.retype {σ : Subst s1 s2}
   induction ht generalizing s2
   case var hb => apply ρ.var _ _ hb
   case sub hsub _ ih =>
-    apply sub
-    { apply hsub.retype ρ }
-    { apply ih ρ }
-  case abs ih =>
-    apply HasType.abs
-    simp [Ty.subst_succVar_comm_base]
-    apply ih ρ.liftVar
-  case tabs ih =>
-    apply HasType.tabs
-    apply ih ρ.liftTVar
-  case app ih1 ih2 =>
-    apply HasType.app
-    { apply ih1 ρ }
-    { apply ih2 ρ }
-  case tapp ih =>
-    simp [Ty.open_tvar_subst_comm]
-    apply HasType.tapp
-    apply ih ρ
+    apply sub <;> try aesop
+    apply hsub.retype ρ
+  case abs ih => apply HasType.abs; simpa [Ty.subst_succVar_comm_base] using ih ρ.liftVar
+  case tabs ih => apply HasType.tabs; apply ih ρ.liftTVar
+  case app ih1 ih2 => apply HasType.app <;> aesop
+  case tapp ih => simp [Ty.open_tvar_subst_comm]; apply HasType.tapp; aesop
