Cslib/Computability/LambdaCalculus/WellScoped/FSub/TypeSoundness/Canonical.lean
@@ -1,132 +1,79 @@
+/-
+# Canonical forms lemmas for System F<:
+-/
+
 import Cslib.Computability.LambdaCalculus.WellScoped.FSub.TypeSystem
 import Cslib.Computability.LambdaCalculus.WellScoped.FSub.RetypeTheory.TypeSystem
 
+/-- Predicate for empty contexts -/
 inductive Ctx.IsEmpty : Ctx s -> Prop where
 | empty_is_empty : Ctx.IsEmpty .empty
 
 theorem HasType.app_inv
   (ht : HasType Γ (.app e1 e2) T) :
   ∃ T1 T2,
-    HasType Γ e1 (.arrow T1 T2)
-    ∧ HasType Γ e2 T1
-    ∧ Subtyp Γ T2 T := by
+    HasType Γ e1 (.arrow T1 T2) ∧ HasType Γ e2 T1 ∧ Subtyp Γ T2 T := by
   generalize he0 : Exp.app e1 e2 = e at ht
-  induction ht <;> cases he0
-  case app T1 U1 _ ht1 ht2 _ _ =>
-    use T1, U1
-    split_ands
-    { exact ht1 }
-    { exact ht2 }
-    { apply Subtyp.refl }
-  case sub hsub _ ih =>
-    have ⟨T1, T2, ht1, ht2, hs0⟩ := ih rfl
-    use T1, T2
-    split_ands
-    { exact ht1 }
-    { exact ht2 }
-    { apply Subtyp.trans hs0 hsub }
+  induction ht <;> cases he0 <;> grind
 
 theorem Subtyp.top_inv
   (hsub : Subtyp Γ .top T) :
   T = .top := by
   generalize he0 : Ty.top = T at hsub
-  induction hsub <;> cases he0
-  case top => rfl
-  case refl => rfl
-  case trans => aesop
+  induction hsub <;> cases he0 <;> try (solve | rfl | aesop)
 
 theorem Subtyp.arrow_inv_left
   (hsub : Subtyp Γ (.arrow T1 U1) T) :
   (∃ T2 U2, T = .arrow T2 U2) ∨ T = .top := by
   generalize he0 : Ty.arrow T1 U1 = T at hsub
-  induction hsub <;> cases he0
-  case top => right; rfl
-  case refl => left; aesop
-  case arrow => left; aesop
+  induction hsub <;> cases he0 <;> try (solve | rfl | aesop)
   case trans ih1 _ ih2 =>
-    specialize ih2 rfl
-    cases ih2
-    case inl ih2 =>
-      aesop
-    case inr ih2 =>
-      cases ih2
-      rename_i hsub _
-      have heq := Subtyp.top_inv hsub
-      aesop
+    cases (ih2 rfl)
+    case inl ih2 => aesop
+    case inr ih2 => cases ih2; grind [Subtyp.top_inv]
 
 theorem Subtyp.poly_inv_left
   (hsub : Subtyp Γ (.poly T1 T2) T) :
   (∃ T3 T4, T = .poly T3 T4) ∨ T = .top := by
   generalize he0 : Ty.poly T1 T2 = T at hsub
-  induction hsub <;> cases he0
-  case top => right; rfl
-  case refl => left; aesop
-  case poly => left; aesop
+  induction hsub <;> cases he0 <;> try (solve | aesop)
   case trans ih1 _ ih2 =>
-    specialize ih2 rfl
-    cases ih2
-    case inl ih2 =>
-      aesop
-    case inr ih2 =>
-      cases ih2
-      rename_i hsub _
-      have heq := Subtyp.top_inv hsub
-      aesop
+    cases (ih2 rfl)
+    case inl ih2 => aesop
+    case inr ih2 => cases ih2; grind [Subtyp.top_inv]
 
 theorem Subtype.tvar_inv_right
   (hsub : Subtyp Γ T (.tvar X)) :
   ∃ X0, T = .tvar X0 := by
   generalize he0 : Ty.tvar X = T0 at hsub
-  induction hsub <;> cases he0
-  case refl => aesop
-  case trans => aesop
-  case tvar => aesop
+  induction hsub <;> cases he0 <;> try (solve | aesop)
 
 theorem Subtyp.arrow_inv_right
   (hsub : Subtyp Γ T (.arrow T2 U2)) :
   (∃ T1 U1, T = .arrow T1 U1) ∨ (∃ X, T = .tvar X) := by
   generalize he0 : Ty.arrow T2 U2 = T0 at hsub
-  induction hsub <;> cases he0
-  case refl => aesop
-  case tvar => aesop
-  case arrow => aesop
+  induction hsub <;> cases he0 <;> try (solve | aesop)
   case trans ih1 _ ih2 =>
-    specialize ih2 rfl
-    cases ih2
+    cases (ih2 rfl)
     case inl ih2 =>
       have ⟨T2, U2, h⟩ := ih2
-      cases h
-      specialize ih1 rfl
-      aesop
+      cases h; specialize ih1 rfl; grind
     case inr ih2 =>
-      have ⟨X, h⟩ := ih2
-      cases h
-      rename_i hsub _
-      have := Subtype.tvar_inv_right hsub
-      aesop
+      have ⟨X, h⟩ := ih2; cases h; rename_i hsub _ _
+      have := Subtype.tvar_inv_right hsub; grind
 
 theorem Subtyp.poly_inv_right
   (hsub : Subtyp Γ T (.poly T2 U2)) :
   (∃ T1 U1, T = .poly T1 U1) ∨ (∃ X, T = .tvar X) := by
   generalize he0 : Ty.poly T2 U2 = T0 at hsub
-  induction hsub <;> cases he0
-  case refl => aesop
-  case tvar => aesop
-  case poly => aesop
+  induction hsub <;> cases he0 <;> try (solve | aesop)
   case trans ih1 _ ih2 =>
-    specialize ih2 rfl
-    cases ih2
-    case inl ih2 =>
-      have ⟨T2, U2, h⟩ := ih2
-      cases h
-      specialize ih1 rfl
-      aesop
+    cases (ih2 rfl)
+    case inl ih2 => have ⟨T2, U2, h⟩ := ih2; cases h; grind
     case inr ih2 =>
-      have ⟨X, h⟩ := ih2
-      cases h
-      rename_i hsub _
-      have := Subtype.tvar_inv_right hsub
-      aesop
+      have ⟨X, h⟩ := ih2; cases h
+      rename_i hsub _ _
+      have := Subtype.tvar_inv_right hsub; grind
 
 theorem Subtyp.arrow_inv
   (hsub : Subtyp Γ (.arrow T1 U1) (.arrow T2 U2)) :
@@ -135,24 +82,8 @@ theorem Subtyp.arrow_inv
   generalize he2 : Ty.arrow T2 U2 = P2 at hsub
   induction hsub <;> cases he1 <;> cases he2
   case refl => constructor <;> apply Subtyp.refl
-  case trans hs1 ih1 hs2 ih2 =>
-    have := Subtyp.arrow_inv_left hs1
-    cases this
-    case inr h =>
-      cases h
-      have := Subtyp.top_inv hs2
-      contradiction
-    case inl h =>
-      have ⟨T3, U3, h⟩ := h
-      cases h
-      specialize ih1 rfl rfl
-      specialize ih2 rfl rfl
-      have ⟨ih11, ih12⟩ := ih1
-      have ⟨ih21, ih22⟩ := ih2
-      constructor
-      { apply Subtyp.trans ih21 ih11 }
-      { apply Subtyp.trans ih12 ih22 }
   case arrow => aesop
+  case trans hs1 ih1 hs2 ih2 => cases (Subtyp.arrow_inv_left hs1) <;> grind [Subtyp.top_inv]
 
 theorem Subtyp.poly_inv
   (hsub : Subtyp Γ (.poly T1 U1) (.poly T2 U2)) :
@@ -163,51 +94,28 @@ theorem Subtyp.poly_inv
   case refl => constructor <;> apply Subtyp.refl
   case poly => aesop
   case trans hs1 ih1 hs2 ih2 =>
-    have := Subtyp.poly_inv_left hs1
-    cases this
+    cases (Subtyp.poly_inv_left hs1)
     case inl h =>
-      have ⟨T3, T4, h⟩ := h
-      cases h
-      specialize ih1 rfl rfl
-      specialize ih2 rfl rfl
-      have ⟨ih11, ih12⟩ := ih1
-      have ⟨ih21, ih22⟩ := ih2
+      have ⟨T3, T4, h⟩ := h; cases h
+      have ⟨ih11, ih12⟩ := ih1 rfl rfl; have ⟨ih21, ih22⟩ := ih2 rfl rfl
       constructor
-      { apply Subtyp.trans ih21 ih11 }
+      { grind }
       { have ih12' := ih12.retype (Retype.narrow_tvar ih21)
-        simp [Ty.subst_id] at ih12'
-        apply Subtyp.trans ih12' ih22 }
-    case inr h =>
-      cases h
-      have := Subtyp.top_inv hs2
-      contradiction
+        grind [Ty.subst_id] }
+    case inr h => cases h; grind [Subtyp.top_inv]
 
 theorem Subtyp.non_tvar_left_inv
   (hsub : Subtyp Γ T1 T2)
   (hnt : ∀ X, T1 ≠ .tvar X) :
   ∀ X, T2 ≠ .tvar X := by
-  induction hsub
-  case top => aesop
-  case refl => aesop
-  case tvar =>
-    rename_i X _ _
-    specialize hnt X
-    contradiction
-  case trans ih1 ih2 => aesop
-  case arrow => aesop
-  case poly => aesop
+  induction hsub <;> try (solve | aesop)
 
 theorem HasType.value_typing
   (hv : Exp.IsVal v)
   (ht : HasType Γ v T) :
   ∀ X, T ≠ .tvar X := by
-  induction ht <;> try (solve | cases hv)
-  case sub hsub _ ih =>
-    specialize ih hv
-    apply Subtyp.non_tvar_left_inv hsub
-    exact ih
-  case abs => aesop
-  case tabs => aesop
+  induction ht <;> try (solve | cases hv | aesop)
+  case sub hsub _ _ => apply Subtyp.non_tvar_left_inv hsub; aesop
 
 theorem HasType.abs_inv {Γ : Ctx s}
   (ht : HasType Γ (.abs T0 e) (.arrow T1 U1)) :
@@ -218,32 +126,11 @@ theorem HasType.abs_inv {Γ : Ctx s}
   generalize he1 : Exp.abs T0 e = t at ht
   generalize he2 : Ty.arrow T1 U1 = P at ht
   induction ht <;> cases he1 <;> cases he2
-  case abs T0 t0 U0 ht _ =>
-    use U0
-    split_ands
-    { exact ht }
-    { apply Subtyp.refl }
-    { apply Subtyp.refl }
+  case abs T0 t0 U0 ht _ => use U0; split_ands <;> grind
   case sub hsub =>
-    have := Subtyp.arrow_inv_right hsub
-    cases this
-    case inl h =>
-      have ⟨T1, U1, h⟩ := h
-      cases h
-      rename_i ih
-      specialize ih rfl rfl
-      have ⟨U0, ih1, ih2, ih3⟩ := ih
-      have ⟨h1, h2⟩ := Subtyp.arrow_inv hsub
-      use U0
-      split_ands
-      { exact ih1 }
-      { apply Subtyp.trans h1 ih2 }
-      { apply Subtyp.trans ih3 h2 }
-    case inr h =>
-      have ⟨X, h⟩ := h
-      rename_i hv _ _
-      have := HasType.value_typing (by constructor) hv
-      aesop
+    cases (Subtyp.arrow_inv_right hsub)
+    case inl h => have ⟨T1, U1, h⟩ := h; cases h; grind [Subtyp.arrow_inv]
+    case inr h => grind [HasType.value_typing]
 
 theorem HasType.tapp_inv
   (ht : HasType Γ (.tapp e T) U) :
@@ -251,20 +138,7 @@ theorem HasType.tapp_inv
     HasType Γ e (.poly T T2)
     ∧ Subtyp Γ (T2.open_tvar T) U := by
   generalize he1 : Exp.tapp e T = t0 at ht
-  induction ht <;> cases he1
-  case tapp =>
-    rename_i T2 ht _
-    use T2
-    split_ands
-    { exact ht }
-    { apply Subtyp.refl }
-  case sub hs _ ih =>
-    specialize ih rfl
-    have ⟨T2, ih1, ih2⟩ := ih
-    use T2
-    split_ands
-    { exact ih1 }
-    { apply Subtyp.trans ih2 hs }
+  induction ht <;> cases he1 <;> grind
 
 theorem HasType.tabs_inv
   (ht : HasType Γ (.tabs T0 e) (.poly T1 U1)) :
@@ -275,78 +149,37 @@ theorem HasType.tabs_inv
   generalize he1 : Exp.tabs T0 e = t0 at ht
   generalize he2 : Ty.poly T1 U1 = P at ht
   induction ht <;> cases he1 <;> cases he2
-  case tabs T _ U h _ =>
-    use U
-    split_ands
-    { exact h }
-    { apply Subtyp.refl }
-    { apply Subtyp.refl }
+  case tabs T _ U h _ => use U; split_ands <;> grind
   case sub ht ih hs =>
-    have := Subtyp.poly_inv_right hs
-    cases this
+    cases (Subtyp.poly_inv_right hs)
     case inl h =>
       have ⟨T2, U2, h⟩ := h
-      cases h
-      rename_i ih
-      specialize ih rfl rfl
-      have ⟨U0, ih1, ih2, ih3⟩ := ih
+      cases h; rename_i ih
+      have ⟨U0, ih1, ih2, ih3⟩ := ih rfl rfl
       have ⟨h1, h2⟩ := Subtyp.poly_inv hs
-      use U0
-      split_ands
-      { exact ih1 }
-      { apply Subtyp.trans h1 ih2 }
+      use U0; split_ands <;> try grind
       { have ih3' := ih3.retype (Retype.narrow_tvar h1)
-        simp [Ty.subst_id] at ih3'
-        apply Subtyp.trans ih3' h2 }
-    case inr h =>
-      have ⟨X, h⟩ := h
-      cases h
-      rename_i ht _
-      have := HasType.value_typing (by constructor) ht
-      aesop
+        grind [Ty.subst_id] }
+    case inr h => grind [HasType.value_typing]
 
 theorem HasType.value_typing_arrow_inv
-  (hv : Exp.IsVal v)
-  (ht : HasType Γ v (.arrow T U)) :
+  (hv : Exp.IsVal v) (ht : HasType Γ v (.arrow T U)) :
   ∃ T0 e0, v = .abs T0 e0 := by
   generalize he : Ty.arrow T U = P at ht
-  induction ht <;> try (solve | cases he | cases hv)
+  induction ht <;> try (solve | cases he | cases hv | aesop)
   case sub ih =>
-    cases he
-    rename_i hs
-    have := Subtyp.arrow_inv_right hs
-    cases this
-    case inl h =>
-      have ⟨T1, U1, h⟩ := h
-      cases h
-      specialize ih hv rfl
-      trivial
-    case inr h =>
-      have ⟨X, h⟩ := h
-      rename_i hvt _
-      have := HasType.value_typing hv hvt
-      aesop
-  case abs => aesop
+    cases he; rename_i hs
+    cases (Subtyp.arrow_inv_right hs)
+    case inl h => aesop
+    case inr h => grind [HasType.value_typing]
 
 theorem HasType.value_typing_poly_inv
-  (hv : Exp.IsVal v)
-  (ht : HasType Γ v (.poly T U)) :
+  (hv : Exp.IsVal v) (ht : HasType Γ v (.poly T U)) :
   ∃ T0 e0, v = .tabs T0 e0 := by
   generalize he : Ty.poly T U = P at ht
-  induction ht <;> try (solve | cases he | cases hv)
+  induction ht <;> try (solve | cases he | cases hv | aesop)
   case sub ih =>
-    cases he
-    rename_i hs
-    have := Subtyp.poly_inv_right hs
-    cases this
-    case inl h =>
-      have ⟨T1, U1, h⟩ := h
-      cases h
-      specialize ih hv rfl
-      trivial
-    case inr h =>
-      have ⟨X, h⟩ := h
-      rename_i hvt _
-      have := HasType.value_typing hv hvt
-      aesop
-  case tabs => aesop
+    cases he; rename_i hs
+    cases (Subtyp.poly_inv_right hs)
+    case inl h => aesop
+    case inr h => grind [HasType.value_typing]
